Struct/DevTest.lean
@@ -1,266 +1,1193 @@
-import Struct.Struct
-
-set_option pp.rawOnError true
-set_option trace.debug true
-
--- Try to get LoVe Hoare logic definition and lemma to Lean 4
-
-example (n : Nat) : n = n := by
-  -- suggests
-  induction n with
-  | zero => sorry
-  | succ n_1 n_1.ih => sorry
-
-namespace LoVe
-
-def state : Type :=
-  String → Nat
-def state.update (name : String) (val : Nat) (s : state) : state := 
-  fun name' => if name' = name then val else s name'
-notation s " { " name " ↦ " val " } " => state.update name val s
-
-inductive stmt : Type
-| skip   : stmt
-| assign : String → (state → Nat) → stmt
-| seq    : stmt → stmt → stmt
-| ite    : (state → Prop) → stmt → stmt → stmt
-| while_tmp  : (state → Prop) → stmt → stmt
-infixl:90 " ;; " => stmt.seq
-
-inductive big_step : stmt → state → state → Prop
-| skip {s} :
-  big_step stmt.skip s s
-| assign {x a s} :
-  big_step (stmt.assign x a) s (s{x ↦ a s})
-| seq {S T s t u} (hS : big_step S s t)
-    (hT : big_step T t u) :
-  big_step (S ;; T) s u
-| ite_true {b : state → Prop} {S T s t} (hcond : b s)
-    (hbody : big_step S s t) :
-  big_step (stmt.ite b S T) s t
-| ite_false {b : state → Prop} {S T s t} (hcond : ¬ b s)
-    (hbody : big_step T s t) :
-  big_step (stmt.ite b S T) s t
-| while_true {b : state → Prop} {S s t u} (hcond : b s)
-    (hbody : big_step S s t)
-    (hrest : big_step (stmt.while_tmp b S) t u) :
-  big_step (stmt.while_tmp b S) s u
-| while_false {b : state → Prop} {S s} (hcond : ¬ b s) :
-  big_step (stmt.while_tmp b S) s s
-infix:110 " ⟹ " => big_step
-
--- NOTE: cannot do induction on hl if it's made with stmt × state and infix ⟹
--- Then we get error `index in target type not a variable, (S, s)`
-theorem big_step_deterministic {S s l r} (hl : big_step S s l) (hr : big_step S s r) : l = r := by
-  induction hl 
-  case skip => 
-    cases hr
-    rfl
-  case assign =>
-    cases hr
-    rfl
-  case seq S T s t l hS hT ihS ihT =>
-    cases hr
-    admit -- TODO
-  case ite_true b S T s t hb hS ih =>
-    cases hr
-    case ite_true x1 x2 x3 x4 => 
-      apply ih x4 -- In lean 3, after using `cases' hr`, they still use `hr` at the underscore. In Lean 4 `hr` does not exist anymore
-    case ite_false =>
-      admit -- cc
-  case ite_false b S T s t hb hT ih =>
-    cases hr
-    case ite_true =>
-      admit -- cc
-    case ite_false x1 x2 x3 x4 =>
-      apply ih x4
-  case while_true b S s t u hb hS hw ihS ihw =>
-    cases hr
-    case while_true x1 x2 x3 x4 x5 x6 =>
-      admit -- bit weird 
-      -- cases ihS _
-      -- cases ihw _
-      -- rfl
-    case while_false =>
-      admit -- cc
-  case while_false =>
-    cases hr
-    case while_true =>
-      admit -- cc
-    case while_false =>
-      rfl
-
-@[simp] theorem big_step_skip_iff {s t} : big_step stmt.skip s t ↔ t = s := by
-  apply Iff.intro
-  case mp =>
-    intro h
-    cases h with
-    | skip => rfl
-  case mpr =>
-    intro h
-    admit
-    --exact big_step.skip _ _
+-- /-
+-- Copyright (c) 2020 Microsoft Corporation. All rights reserved.
+-- Released under Apache 2.0 license as described in the file LICENSE.
+-- Authors: Leonardo de Moura, Sebastian Ullrich
+-- -/
 
 
--- def partial_hoare (P : state → Prop) (S : stmt) (Q : state → Prop) : Prop := 
---   ∀ s t, P s → (S, s) ⟹ t → Q t
 
--- notation:110 " {* " P " *} " S " {* " Q " *} " => partial_hoare P S Q
 
--- theorem skip_intro {P : state → Prop} : {* P *} stmt.skip {* P *} := by
---   rw [partial_hoare]
---   intros s t hs hst
---   cases hst
---   assumption
+-- namespace Lean.Elab.Tactic
+-- open Meta
 
--- def while_intro (P : state → Prop) {b : state → Prop} {S}
---   (h : {* fun s => P s ∧ b s *} S {* P *}) :
---   {* P *} stmt.while_tmp b S {* fun s => P s ∧ ¬ b s *} := by
---     intros s t hs hst
+-- /-
+--   Given an `inductionAlt` of the form
+--   ```
+--   syntax inductionAltLHS := "| " (group("@"? ident) <|> hole) (ident <|> hole)*
+--   syntax inductionAlt  := ppDedent(ppLine) inductionAltLHS+ " => " (hole <|> syntheticHole <|> tacticSeq)
+--   ```
+-- -/
+-- private def getFirstAltLhs (alt : Syntax) : Syntax :=
+--   alt[0][0]
+-- /-- Return `inductionAlt` name. It assumes `alt` does not have multiple `inductionAltLHS` -/
+-- private def getAltName (alt : Syntax) : Name :=
+--   let lhs := getFirstAltLhs alt
+--   if !lhs[1].isOfKind ``Parser.Term.hole then lhs[1][1].getId.eraseMacroScopes else `_
+-- /-- Return `true` if the first LHS of the given alternative contains `@`. -/
+-- private def altHasExplicitModifier (alt : Syntax) : Bool :=
+--   let lhs := getFirstAltLhs alt
+--   !lhs[1].isOfKind ``Parser.Term.hole && !lhs[1][0].isNone
+-- /-- Return the variables in the first LHS of the given alternative. -/
+-- private def getAltVars (alt : Syntax) : Array Syntax :=
+--   let lhs := getFirstAltLhs alt
+--   lhs[2].getArgs
+-- /-- Return the variable names in the first LHS of the given alternative. -/
+-- private def getAltVarNames (alt : Syntax) : Array Name :=
+--   getAltVars  alt |>.map getNameOfIdent'
+-- private def getAltRHS (alt : Syntax) : Syntax :=
+--   alt[2]
+-- private def getAltDArrow (alt : Syntax) : Syntax :=
+--   alt[1]
+
+-- -- Return true if `stx` is a term occurring in the RHS of the induction/cases tactic
+-- def isHoleRHS (rhs : Syntax) : Bool :=
+--   rhs.isOfKind ``Parser.Term.syntheticHole || rhs.isOfKind ``Parser.Term.hole
+
+-- def evalAlt (mvarId : MVarId) (alt : Syntax) (remainingGoals : Array MVarId) : TacticM (Array MVarId) :=
+--   let rhs := getAltRHS alt
+--   withCaseRef (getAltDArrow alt) rhs do
+--     if isHoleRHS rhs then
+--       let gs' ← mvarId.withContext <| withRef rhs do
+--         let mvarDecl ← mvarId.getDecl
+--         let val ← elabTermEnsuringType rhs mvarDecl.type
+--         mvarId.assign val
+--         let gs' ← getMVarsNoDelayed val
+--         tagUntaggedGoals mvarDecl.userName `induction gs'.toList
+--         pure gs'
+--       return remainingGoals ++ gs'
+--     else
+--       setGoals [mvarId]
+--       closeUsingOrAdmit (withTacticInfoContext alt (evalTactic rhs))
+--       return remainingGoals
+
+-- /-!
+--   Helper method for creating an user-defined eliminator/recursor application.
+-- -/
+-- namespace ElimApp
+
+-- structure Context where
+--   elimInfo : ElimInfo
+--   targets  : Array Expr -- targets provided by the user
+
+-- structure State where
+--   argPos    : Nat := 0 -- current argument position
+--   targetPos : Nat := 0 -- current target at targetsStx
+--   f         : Expr
+--   fType     : Expr
+--   alts      : Array (Name × MVarId) := #[]
+--   insts     : Array MVarId := #[]
+
+-- abbrev M := ReaderT Context $ StateRefT State TermElabM
+
+-- private def addNewArg (arg : Expr) : M Unit :=
+--   modify fun s => { s with argPos := s.argPos+1, f := mkApp s.f arg, fType := s.fType.bindingBody!.instantiate1 arg }
+
+-- /-- Return the binder name at `fType`. This method assumes `fType` is a function type. -/
+-- private def getBindingName : M Name := return (← get).fType.bindingName!
+-- /-- Return the next argument expected type. This method assumes `fType` is a function type. -/
+-- private def getArgExpectedType : M Expr := return (← get).fType.bindingDomain!
+
+-- private def getFType : M Expr := do
+--   let fType ← whnfForall (← get).fType
+--   modify fun s => { s with fType := fType }
+--   pure fType
+
+-- structure Result where
+--   elimApp : Expr
+--   alts    : Array (Name × MVarId) := #[]
+--   others  : Array MVarId := #[]
+
+-- /--
+--   Construct the an eliminator/recursor application. `targets` contains the explicit and implicit targets for
+--   the eliminator. For example, the indices of builtin recursors are considered implicit targets.
+--   Remark: the method `addImplicitTargets` may be used to compute the sequence of implicit and explicit targets
+--   from the explicit ones.
+-- -/
+-- partial def mkElimApp (elimInfo : ElimInfo) (targets : Array Expr) (tag : Name) : TermElabM Result := do
+--   let rec loop : M Unit := do
+--     match (← getFType) with
+--     | .forallE binderName _ _ c =>
+--       let ctx ← read
+--       let argPos := (← get).argPos
+--       if ctx.elimInfo.motivePos == argPos then
+--         let motive ← mkFreshExprMVar (← getArgExpectedType) MetavarKind.syntheticOpaque
+--         addNewArg motive
+--       else if ctx.elimInfo.targetsPos.contains argPos then
+--         let s ← get
+--         let ctx ← read
+--         unless s.targetPos < ctx.targets.size do
+--           throwError "insufficient number of targets for '{elimInfo.name}'"
+--         let target := ctx.targets[s.targetPos]!
+--         let expectedType ← getArgExpectedType
+--         let target ← withAssignableSyntheticOpaque <| Term.ensureHasType expectedType target
+--         modify fun s => { s with targetPos := s.targetPos + 1 }
+--         addNewArg target
+--       else match c with
+--         | .implicit =>
+--           let arg ← mkFreshExprMVar (← getArgExpectedType)
+--           addNewArg arg
+--         | .strictImplicit =>
+--           let arg ← mkFreshExprMVar (← getArgExpectedType)
+--           addNewArg arg
+--         | .instImplicit =>
+--           let arg ← mkFreshExprMVar (← getArgExpectedType) (kind := MetavarKind.synthetic) (userName := appendTag tag binderName)
+--           modify fun s => { s with insts := s.insts.push arg.mvarId! }
+--           addNewArg arg
+--         | _ =>
+--           let arg ← mkFreshExprSyntheticOpaqueMVar (← getArgExpectedType) (tag := appendTag tag binderName)
+--           let x   ← getBindingName
+--           modify fun s => { s with alts := s.alts.push (x, arg.mvarId!) }
+--           addNewArg arg
+--       loop
+--     | _ =>
+--       pure ()
+--   let f ← Term.mkConst elimInfo.name
+--   let fType ← inferType f
+--   let (_, s) ← (loop).run { elimInfo := elimInfo, targets := targets } |>.run { f := f, fType := fType }
+--   let mut others := #[]
+--   for mvarId in s.insts do
+--     try
+--       unless (← Term.synthesizeInstMVarCore mvarId) do
+--         mvarId.setKind .syntheticOpaque
+--         others := others.push mvarId
+--     catch _ =>
+--       mvarId.setKind .syntheticOpaque
+--       others := others.push mvarId
+--   let alts ← s.alts.filterM fun alt => return !(← alt.2.isAssigned)
+--   return { elimApp := (← instantiateMVars s.f), alts, others := others }
+
+-- /-- Given a goal `... targets ... |- C[targets]` associated with `mvarId`, assign
+--   `motiveArg := fun targets => C[targets]` -/
+-- def setMotiveArg (mvarId : MVarId) (motiveArg : MVarId) (targets : Array FVarId) : MetaM Unit := do
+--   let type ← inferType (mkMVar mvarId)
+--   let motive ← mkLambdaFVars (targets.map mkFVar) type
+--   let motiverInferredType ← inferType motive
+--   let motiveType ← inferType (mkMVar motiveArg)
+--   unless (← isDefEqGuarded motiverInferredType motiveType) do
+--     throwError "type mismatch when assigning motive{indentExpr motive}\n{← mkHasTypeButIsExpectedMsg motiverInferredType motiveType}"
+--   motiveArg.assign motive
+
+-- private def getAltNumFields (elimInfo : ElimInfo) (altName : Name) : TermElabM Nat := do
+--   for altInfo in elimInfo.altsInfo do
+--     if altInfo.name == altName then
+--       return altInfo.numFields
+--   throwError "unknown alternative name '{altName}'"
+
+-- private def checkAltNames (alts : Array (Name × MVarId)) (altsSyntax : Array Syntax) : TacticM Unit :=
+--   for i in [:altsSyntax.size] do
+--     let altStx := altsSyntax[i]!
+--     if getAltName altStx == `_ && i != altsSyntax.size - 1 then
+--       withRef altStx <| throwError "invalid occurrence of wildcard alternative, it must be the last alternative"
+--     let altName := getAltName altStx
+--     if altName != `_ then
+--       unless alts.any fun (n, _) => n == altName do
+--         throwErrorAt altStx "invalid alternative name '{altName}'"
+
+-- /-- Given the goal `altMVarId` for a given alternative that introduces `numFields` new variables,
+--     return the number of explicit variables. Recall that when the `@` is not used, only the explicit variables can
+--     be named by the user. -/
+-- private def getNumExplicitFields (altMVarId : MVarId) (numFields : Nat) : MetaM Nat := altMVarId.withContext do
+--   let target ← altMVarId.getType
+--   withoutModifyingState do
+--     let (_, bis, _) ← forallMetaBoundedTelescope target numFields
+--     return bis.foldl (init := 0) fun r bi => if bi.isExplicit then r + 1 else r
+
+-- private def saveAltVarsInfo (altMVarId : MVarId) (altStx : Syntax) (fvarIds : Array FVarId) : TacticM Unit :=
+--   withSaveInfoContext <| altMVarId.withContext do
+--     let useNamesForExplicitOnly := !altHasExplicitModifier altStx
+--     let mut i := 0
+--     let altVars := getAltVars altStx
+--     for fvarId in fvarIds do
+--       if !useNamesForExplicitOnly || (← fvarId.getDecl).binderInfo.isExplicit then
+--         if i < altVars.size then
+--           Term.addLocalVarInfo altVars[i]! (mkFVar fvarId)
+--           i := i + 1
+
+-- /--
+--   If `altsSyntax` is not empty we reorder `alts` using the order the alternatives have been provided
+--   in `altsSyntax`. Motivations:
+
+--   1- It improves the effectiveness of the `checkpoint` and `save` tactics. Consider the following example:
+--   ```lean
+--   example (h₁ : p ∨ q) (h₂ : p → x = 0) (h₃ : q → y = 0) : x * y = 0 := by
+--     cases h₁ with
+--     | inr h =>
+--       sleep 5000 -- sleeps for 5 seconds
+--       save
+--       have : y = 0 := h₃ h
+--       -- We can confortably work here
+--     | inl h => stop ...
+--   ```
+--   If we do reorder, the `inl` alternative will be executed first. Moreover, as we type in the `inr` alternative,
+--   type errors will "swallow" the `inl` alternative and affect the tactic state at `save` making it ineffective.
+
+--   2- The errors are produced in the same order the appear in the code above. This is not super important when using IDEs.
+-- -/
+-- def reorderAlts (alts : Array (Name × MVarId)) (altsSyntax : Array Syntax) : Array (Name × MVarId) := Id.run do
+--   if altsSyntax.isEmpty then
+--     return alts
+--   else
+--     let mut alts := alts
+--     let mut result := #[]
+--     for altStx in altsSyntax do
+--       let altName := getAltName altStx
+--       let some i := alts.findIdx? (·.1 == altName) | return result ++ alts
+--       result := result.push alts[i]!
+--       alts := alts.eraseIdx i
+--     return result ++ alts
+
+-- -- TODO: Change myEvalAlts to return list of MVars
+-- -- `getAltMVars` or something
+-- def myEvalAlts (elimInfo : ElimInfo) (alts : Array (Name × MVarId)) (optPreTac : Syntax) (altsSyntax : Array Syntax)
+--     (initialInfo : Info)
+--     (numEqs : Nat := 0) (numGeneralized : Nat := 0) (toClear : Array FVarId := #[]) : TacticM Unit := do
+--   checkAltNames alts altsSyntax
+--   let hasAlts := altsSyntax.size > 0
+--   if hasAlts then
+--     -- default to initial state outside of alts
+--     withInfoContext go (pure initialInfo)
+--   else go
+-- where
+--   go := do
+--     let alts := reorderAlts alts altsSyntax
+--     let hasAlts := altsSyntax.size > 0
+--     let mut usedWildcard := false
+--     let mut subgoals := #[] -- when alternatives are not provided, we accumulate subgoals here
+--     let mut altsSyntax := altsSyntax
+
+--     -- TODO foreach, add mvar to list
+--     for (altName, altMVarId) in alts do
+--       trace[Elab.induction] "Alternative {altName}"
+--       let numFields ← getAltNumFields elimInfo altName
+--       let mut isWildcard := false
+--       let altStx? ←
+--         match altsSyntax.findIdx? (fun alt => getAltName alt == altName) with
+--         | some idx =>
+--           let altStx := altsSyntax[idx]!
+--           altsSyntax := altsSyntax.eraseIdx idx
+--           pure (some altStx)
+--         | none => match altsSyntax.findIdx? (fun alt => getAltName alt == `_) with
+--           | some idx =>
+--             isWildcard := true
+--             pure (some altsSyntax[idx]!)
+--           | none =>
+--             pure none
+--       match altStx? with
+--       | none =>
+--         -- This is probably a match without any alternative syntax, all intro's are inaccessible anyways
+--         let mut (_, altMVarId) ← altMVarId.introN numFields
+--         match (← Cases.unifyEqs? numEqs altMVarId {}) with
+--         | none   => pure () -- alternative is not reachable
+--         | some (altMVarId', _) =>
+--           (_, altMVarId) ← altMVarId'.introNP numGeneralized
+--           for fvarId in toClear do
+--             altMVarId ← altMVarId.tryClear fvarId
+--           let altMVarIds ← applyPreTac altMVarId
+--           if !hasAlts then
+--             -- User did not provide alternatives using `|`
+--             subgoals := subgoals ++ altMVarIds.toArray
+--           else if altMVarIds.isEmpty then
+--             pure ()
+--           else
+--             logError m!"alternative '{altName}' has not been provided"
+--             altMVarIds.forM fun mvarId => admitGoal mvarId
+--       | some altStx =>
+--         trace[Elab.induction] "After creating altStx, I match on some altStx {altStx}"
+--         (subgoals, usedWildcard) ← withRef altStx do
+--           let unusedAlt :=
+--             if isWildcard then
+--               pure (#[], usedWildcard)
+--             else
+--               throwError "alternative '{altName}' is not needed"
+--           let altVarNames := getAltVarNames altStx
+--           let numFieldsToName ← if altHasExplicitModifier altStx then pure numFields else getNumExplicitFields altMVarId numFields
+--           if altVarNames.size > numFieldsToName then
+--             logError m!"too many variable names provided at alternative '{altName}', #{altVarNames.size} provided, but #{numFieldsToName} expected"
+--           let mut (fvarIds, altMVarId) ← altMVarId.introN numFields altVarNames.toList (useNamesForExplicitOnly := !altHasExplicitModifier altStx)
+          
+          
+--           -- NOTE TODO: This is actually the new goal post match statement
+--           trace[Elab.induction] "Test01: {(← instantiateMVars (← altMVarId.getDecl).type)}"
+--           altMVarId.withContext do
+--             for ldecl in (← getLCtx) do
+--               trace[Elab.induction] "Test02, {ldecl.userName}: {(← instantiateMVars ldecl.type)}"        
+
+
+--           saveAltVarsInfo altMVarId altStx fvarIds
+--           match (← Cases.unifyEqs? numEqs altMVarId {}) with
+--           | none => unusedAlt
+--           | some (altMVarId', _) =>
+--             (_, altMVarId) ← altMVarId'.introNP numGeneralized
+--             for fvarId in toClear do
+--               altMVarId ← altMVarId.tryClear fvarId
+--             let altMVarIds ← applyPreTac altMVarId
+--             if altMVarIds.isEmpty then
+--               unusedAlt
+--             else
+--               let mut subgoals := subgoals
+--               for altMVarId' in altMVarIds do
+--                 altMVarId'.withContext do
+--                   trace[Elab.induction] m!"Test03, {(← instantiateMVars (← altMVarId'.getDecl).type)}"
+--                   altMVarId'.withContext do
+--                     for ldecl in (← getLCtx) do
+--                       trace[Elab.induction] "Test04, {ldecl.userName}: {(← instantiateMVars ldecl.type)}"  
+
+
+--                 subgoals ← evalAlt altMVarId' altStx subgoals
+--               pure (subgoals, usedWildcard || isWildcard)          
+--     if usedWildcard then
+--       altsSyntax := altsSyntax.filter fun alt => getAltName alt != `_
+--     unless altsSyntax.isEmpty do
+--       logErrorAt altsSyntax[0]! "unused alternative"
+--     for goal in subgoals do
+--       trace[Elab.induction] m!"TEST: {(← instantiateMVars (← goal.getDecl).type)}"
+--     setGoals subgoals.toList
+--   applyPreTac (mvarId : MVarId) : TacticM (List MVarId) :=
+--     if optPreTac.isNone then do
+--       return [mvarId]
+--     else
+--       evalTacticAt optPreTac[0] mvarId
+
+-- end ElimApp
+
+-- /-
+--   Recall that
+--   ```
+--   generalizingVars := optional (" generalizing " >> many1 ident)
+--   «induction»  := leading_parser nonReservedSymbol "induction " >> majorPremise >> usingRec >> generalizingVars >> optional inductionAlts
+--   ```
+--   `stx` is syntax for `induction`. -/
+-- private def getUserGeneralizingFVarIds (stx : Syntax) : TacticM (Array FVarId) :=
+--   withRef stx do
+--     let generalizingStx := stx[3]
+--     if generalizingStx.isNone then
+--       pure #[]
+--     else
+--       trace[Elab.induction] "{generalizingStx}"
+--       let vars := generalizingStx[1].getArgs
+--       getFVarIds vars
+
+-- -- process `generalizingVars` subterm of induction Syntax `stx`.
+-- private def generalizeVars (mvarId : MVarId) (stx : Syntax) (targets : Array Expr) : TacticM (Nat × MVarId) :=
+--   mvarId.withContext do
+--     let userFVarIds ← getUserGeneralizingFVarIds stx
+--     let forbidden ← mkGeneralizationForbiddenSet targets
+--     let mut s ← getFVarSetToGeneralize targets forbidden
+--     for userFVarId in userFVarIds do
+--       if forbidden.contains userFVarId then
+--         throwError "variable cannot be generalized because target depends on it{indentExpr (mkFVar userFVarId)}"
+--       if s.contains userFVarId then
+--         throwError "unnecessary 'generalizing' argument, variable '{mkFVar userFVarId}' is generalized automatically"
+--       s := s.insert userFVarId
+--     let fvarIds ← sortFVarIds s.toArray
+--     let (fvarIds, mvarId') ← mvarId.revert fvarIds
+--     return (fvarIds.size, mvarId')
+
+-- /--
+-- Given `inductionAlts` of the fom
+-- ```
+-- syntax inductionAlts := "with " (tactic)? withPosition( (colGe inductionAlt)+)
+-- ```
+-- Return an array containing its alternatives.
+-- -/
+-- private def getAltsOfInductionAlts (inductionAlts : Syntax) : Array Syntax :=
+--   inductionAlts[2].getArgs
+
+-- private def getAltsOfOptInductionAlts (optInductionAlts : Syntax) : Array Syntax :=
+--   if optInductionAlts.isNone then #[] else getAltsOfInductionAlts optInductionAlts[0]
+
+-- private def getOptPreTacOfOptInductionAlts (optInductionAlts : Syntax) : Syntax :=
+--   if optInductionAlts.isNone then mkNullNode else optInductionAlts[0][1]
+
+-- private def isMultiAlt (alt : Syntax) : Bool :=
+--   alt[0].getNumArgs > 1
+
+-- /-- Return `some #[alt_1, ..., alt_n]` if `alt` has multiple LHSs. -/
+-- private def expandMultiAlt? (alt : Syntax) : Option (Array Syntax) := Id.run do
+--   if isMultiAlt alt then
+--     some <| alt[0].getArgs.map fun lhs => alt.setArg 0 (mkNullNode #[lhs])
+--   else
+--     none
+
+-- /--
+-- Given `inductionAlts` of the form
+-- ```
+-- syntax inductionAlts := "with " (tactic)? withPosition( (colGe inductionAlt)+)
+-- ```
+-- Return `some inductionAlts'` if one of the alternatives have multiple LHSs, in the new `inductionAlts'`
+-- all alternatives have a single LHS.
+
+-- Remark: the `RHS` of alternatives with multi LHSs is copied.
+-- -/
+-- private def expandInductionAlts? (inductionAlts : Syntax) : Option Syntax := Id.run do
+--   let alts := getAltsOfInductionAlts inductionAlts
+--   if alts.any isMultiAlt then
+--     let mut altsNew := #[]
+--     for alt in alts do
+--       if let some alt' := expandMultiAlt? alt then
+--         altsNew := altsNew ++ alt'
+--       else
+--         altsNew := altsNew.push alt
+--     some <| inductionAlts.setArg 2 (mkNullNode altsNew)
+--   else
+--     none
+
+-- /--
+-- Expand
+-- ```
+-- syntax "induction " term,+ (" using " ident)?  ("generalizing " (colGt term:max)+)? (inductionAlts)? : tactic
+-- ```
+-- if `inductionAlts` has an alternative with multiple LHSs.
+-- -/
+-- private def expandInduction? (induction : Syntax) : Option Syntax := do
+--   let optInductionAlts := induction[4]
+--   guard <| !optInductionAlts.isNone
+--   let inductionAlts' ← expandInductionAlts? optInductionAlts[0]
+--   return induction.setArg 4 (mkNullNode #[inductionAlts'])
+
+-- /--
+-- Expand
+-- ```
+-- syntax "cases " casesTarget,+ (" using " ident)? (inductionAlts)? : tactic
+-- ```
+-- if `inductionAlts` has an alternative with multiple LHSs.
+-- -/
+-- private def expandCases? (induction : Syntax) : Option Syntax := do
+--   let optInductionAlts := induction[3]
+--   guard <| !optInductionAlts.isNone
+--   let inductionAlts' ← expandInductionAlts? optInductionAlts[0]
+--   return induction.setArg 3 (mkNullNode #[inductionAlts'])
+
+-- /--
+--   We may have at most one `| _ => ...` (wildcard alternative), and it must not set variable names.
+--   The idea is to make sure users do not write unstructured tactics. -/
+-- private def checkAltsOfOptInductionAlts (optInductionAlts : Syntax) : TacticM Unit :=
+--   unless optInductionAlts.isNone do
+--     let mut found := false
+--     for alt in getAltsOfInductionAlts optInductionAlts[0] do
+--       let n := getAltName alt
+--       if n == `_ then
+--         unless (getAltVarNames alt).isEmpty do
+--           throwErrorAt alt "wildcard alternative must not specify variable names"
+--         if found then
+--           throwErrorAt alt "more than one wildcard alternative '| _ => ...' used"
+--         found := true
+
+-- def getInductiveValFromMajor (major : Expr) : TacticM InductiveVal :=
+--   liftMetaMAtMain fun mvarId => do
+--     let majorType ← inferType major
+--     let majorType ← whnf majorType
+--     matchConstInduct majorType.getAppFn
+--       (fun _ => Meta.throwTacticEx `induction mvarId m!"major premise type is not an inductive type {indentExpr majorType}")
+--       (fun val _ => pure val)
+
+-- -- `optElimId` is of the form `("using" ident)?`
+-- private def getElimNameInfo (optElimId : Syntax) (targets : Array Expr) (induction : Bool): TacticM ElimInfo := do
+--   if optElimId.isNone then
+--     if let some elimInfo ← getCustomEliminator? targets then
+--       return elimInfo
+--     unless targets.size == 1 do
+--       throwError "eliminator must be provided when multiple targets are used (use 'using <eliminator-name>'), and no default eliminator has been registered using attribute `[eliminator]`"
+--     let indVal ← getInductiveValFromMajor targets[0]!
+--     if induction && indVal.all.length != 1 then
+--       throwError "'induction' tactic does not support mutually inductive types, the eliminator '{mkRecName indVal.name}' has multiple motives"
+--     if induction && indVal.isNested then
+--       throwError "'induction' tactic does not support nested inductive types, the eliminator '{mkRecName indVal.name}' has multiple motives"
+--     let elimName := if induction then mkRecName indVal.name else mkCasesOnName indVal.name
+--     getElimInfo elimName
+--   else
+--     let elimId := optElimId[1]
+--     let elimName ← withRef elimId do resolveGlobalConstNoOverloadWithInfo elimId
+--     withRef elimId <| getElimInfo elimName
+
+-- private def shouldGeneralizeTarget (e : Expr) : MetaM Bool := do
+--   if let .fvar fvarId .. := e then
+--     return (←  fvarId.getDecl).hasValue -- must generalize let-decls
+--   else
+--     return true
+
+-- private def generalizeTargets (exprs : Array Expr) : TacticM (Array Expr) := do
+--   if (← withMainContext <| exprs.anyM (shouldGeneralizeTarget ·)) then
+--     liftMetaTacticAux fun mvarId => do
+--       let (fvarIds, mvarId) ← mvarId.generalize (exprs.map fun expr => { expr })
+--       return (fvarIds.map mkFVar, [mvarId])
+--   else
+--     return exprs
+
+-- def myEvalInduction : Tactic := fun stx =>
+--   match expandInduction? stx with
+--   | some stxNew => withMacroExpansion stx stxNew <| evalTactic stxNew
+--   | _ => focus do
+--     let optInductionAlts := stx[4]
+--     let alts := getAltsOfOptInductionAlts optInductionAlts
+--     let targets ← withMainContext <| stx[1].getSepArgs.mapM (elabTerm · none)
+--     let targets ← generalizeTargets targets
+--     let elimInfo ← withMainContext <| getElimNameInfo stx[2] targets (induction := true)
+--     let mvarId ← getMainGoal
+--     -- save initial info before main goal is reassigned
+--     let initInfo ← mkTacticInfo (← getMCtx) (← getUnsolvedGoals) (← getRef)
+--     let tag ← mvarId.getTag
+--     mvarId.withContext do
+--       let targets ← addImplicitTargets elimInfo targets
+--       checkTargets targets
+--       let targetFVarIds := targets.map (·.fvarId!)
+--       let (n, mvarId) ← generalizeVars mvarId stx targets
+--       mvarId.withContext do
+--         let result ← withRef stx[1] do -- use target position as reference
+--           ElimApp.mkElimApp elimInfo targets tag
+--         trace[Elab.induction] "elimApp: {result.elimApp}"
+        
+--         -- let x ← result.alts.mapM (fun (name, mvar) => do
+--         --   let y ← mvar.getDecl
+--         --   let z ← instantiateMVars y.type
+--         --   trace[Elab.induction] "{name}: {z}"
+--         --   for ldecl in y.lctx do
+--         --     trace[Elab.induction] "alts, {ldecl.userName}: {(← instantiateMVars ldecl.type)}"
+--         --   )
+--         -- let x ← result.others.mapM (fun mvar => do
+--         --   let y ← mvar.getDecl
+--         --   let z ← instantiateMVars y.type
+--         --   trace[Elab.induction] "_: {z}"
+--         --   for ldecl in y.lctx do
+--         --     trace[Elab.induction] "others, {ldecl.userName}: {(← instantiateMVars ldecl.type)}"
+--         --   )
+
+--         let elimArgs := result.elimApp.getAppArgs
+--         ElimApp.setMotiveArg mvarId elimArgs[elimInfo.motivePos]!.mvarId! targetFVarIds
+--         let optPreTac := getOptPreTacOfOptInductionAlts optInductionAlts
+
+--         mvarId.assign result.elimApp
+
+--         -- mvarId.withContext do
+--         --   for ldecl in (← getLCtx) do
+--         --     trace[Elab.induction] "test, {ldecl.userName}: {(← instantiateMVars ldecl.type)}"
+
+--         ElimApp.myEvalAlts elimInfo result.alts optPreTac alts initInfo (numGeneralized := n) (toClear := targetFVarIds)
+--         appendGoals result.others.toList
+-- where
+--   checkTargets (targets : Array Expr) : MetaM Unit := do
+--     let mut foundFVars : FVarIdSet := {}
+--     for target in targets do
+--       unless target.isFVar do
+--         throwError "index in target's type is not a variable (consider using the `cases` tactic instead){indentExpr target}"
+--       if foundFVars.contains target.fvarId! then
+--         throwError "target (or one of its indices) occurs more than once{indentExpr target}"
+
+-- def elabCasesTargets (targets : Array Syntax) : TacticM (Array Expr) :=
+--   withMainContext do
+--     let args ← targets.mapM fun target => do
+--       let hName? := if target[0].isNone then none else some target[0][0].getId
+--       let expr ← elabTerm target[1] none
+--       return { expr, hName? : GeneralizeArg }
+--     if (← withMainContext <| args.anyM fun arg => shouldGeneralizeTarget arg.expr <||> pure arg.hName?.isSome) then
+--       liftMetaTacticAux fun mvarId => do
+--         let argsToGeneralize ← args.filterM fun arg => shouldGeneralizeTarget arg.expr <||> pure arg.hName?.isSome
+--         let (fvarIdsNew, mvarId) ← mvarId.generalize argsToGeneralize
+--         let mut result := #[]
+--         let mut j := 0
+--         for arg in args do
+--           if (← shouldGeneralizeTarget arg.expr) || arg.hName?.isSome then
+--             result := result.push (mkFVar fvarIdsNew[j]!)
+--             j := j+1
+--           else
+--             result := result.push arg.expr
+--         return (result, [mvarId])
+--     else
+--       return args.map (·.expr)
+
+-- def myEvalCases : Tactic := fun stx =>
+--   match expandCases? stx with
+--   | some stxNew => withMacroExpansion stx stxNew <| evalTactic stxNew
+--   | _ => focus do
+--     -- leading_parser nonReservedSymbol "cases " >> sepBy1 (group majorPremise) ", " >> usingRec >> optInductionAlts
+--     let targets ← elabCasesTargets stx[1].getSepArgs
+--     let optInductionAlts := stx[3]
+--     let optPreTac := getOptPreTacOfOptInductionAlts optInductionAlts
+--     let alts :=  getAltsOfOptInductionAlts optInductionAlts
+--     let targetRef := stx[1]
+--     let elimInfo ← withMainContext <| getElimNameInfo stx[2] targets (induction := false)
+--     let mvarId ← getMainGoal
+--     -- save initial info before main goal is reassigned
+--     let initInfo ← mkTacticInfo (← getMCtx) (← getUnsolvedGoals) (← getRef)
+--     let tag ← mvarId.getTag
+--     mvarId.withContext do
+--       let targets ← addImplicitTargets elimInfo targets
+--       let result ← withRef targetRef <| ElimApp.mkElimApp elimInfo targets tag
+--       let elimArgs := result.elimApp.getAppArgs
+--       let targets ← elimInfo.targetsPos.mapM fun i => instantiateMVars elimArgs[i]!
+--       let motiveType ← inferType elimArgs[elimInfo.motivePos]!
+--       let mvarId ← generalizeTargetsEq mvarId motiveType targets
+--       let (targetsNew, mvarId) ← mvarId.introN targets.size
+
+--       mvarId.withContext do
+--         ElimApp.setMotiveArg mvarId elimArgs[elimInfo.motivePos]!.mvarId! targetsNew
+--         mvarId.assign result.elimApp
+--         ElimApp.myEvalAlts elimInfo result.alts optPreTac alts initInfo (numEqs := targets.size) (toClear := targetsNew)
+
+-- builtin_initialize
+--   registerTraceClass `Elab.cases
+--   registerTraceClass `Elab.induction
+
+-- open
+--   Lean.Parser.Tactic
+
+-- elab &"myTestTactic " t:term " : " t2:ident  " : " t3:(ident) : tactic => do
+--   let case1 := mkIdent "zero"
+--   let case2 := mkIdent "succ"
+--   let indAlt1 ← `(inductionAlt| | $case1 => sorry)
+--   let indAlt2 ← `(inductionAlt| | $case2 $t2 $t3 => sorry)
+--   myEvalInduction (← `(tactic|induction $t with $indAlt1:inductionAlt $indAlt2:inductionAlt))
+
+-- elab &"myTestTactic2 " t:casesTarget " : " t2:ident : tactic => do
+--   let case1 := mkIdent "zero"
+--   let case2 := mkIdent "succ"
+--   let indAlt1 ← `(inductionAlt| | $case1 => sorry)
+--   let indAlt2 ← `(inductionAlt| | $case2 $t2 => sorry)
+--   myEvalCases (← `(tactic|cases $t with $indAlt1:inductionAlt $indAlt2:inductionAlt))
+
+
+-- end Lean.Elab.Tactic
+
+
+-- set_option trace.Elab.induction true
+-- set_option pp.rawOnError true
+
+-- example (n : Nat) : n = n := by
+--   -- Q : Why do goals contain _uniq, even if the relevant mvar seems named in ldecls?
+--   myTestTactic (n) : m : m.ih 
+--   -- myTestTactic2 (n) : m
+--   -- cases n with
+--   -- | zero => sorry
+--   -- | succ m => sorry
+--   -- repeat admit
+
+
+import Lean.Util.CollectFVars
+import Lean.Parser.Term
+import Lean.Meta.RecursorInfo
+import Lean.Meta.CollectMVars
+import Lean.Meta.Tactic.ElimInfo
+import Lean.Meta.Tactic.Induction
+import Lean.Meta.Tactic.Cases
+import Lean.Meta.GeneralizeVars
+import Lean.Elab.App
+import Lean.Elab.Tactic.ElabTerm
+import Lean.Elab.Tactic.Generalize
+
+namespace InductionHelper
+
+open 
+  Lean 
+  Lean.Expr
+  Lean.Meta 
+  Lean.Elab
+  Lean.Elab.Tactic
+  Lean.PrettyPrinter 
+
+-- # Necessary duplicate (private) helper functions from Lean.Elab.Tactic.induction from nightly-2022-08-09
+-- # Removed most comments, removed namespaces
+private def getFirstAltLhs (alt : Syntax) : Syntax :=
+  alt[0][0]
+private def getAltName (alt : Syntax) : Name :=
+  let lhs := getFirstAltLhs alt
+  if !lhs[1].isOfKind ``Parser.Term.hole then lhs[1][1].getId.eraseMacroScopes else `_
+private def altHasExplicitModifier (alt : Syntax) : Bool :=
+  let lhs := getFirstAltLhs alt
+  !lhs[1].isOfKind ``Parser.Term.hole && !lhs[1][0].isNone
+private def getAltVars (alt : Syntax) : Array Syntax :=
+  let lhs := getFirstAltLhs alt
+  lhs[2].getArgs
+private def getAltVarNames (alt : Syntax) : Array Name :=
+  getAltVars  alt |>.map getNameOfIdent'
+private def getAltRHS (alt : Syntax) : Syntax :=
+  alt[2]
+private def getAltDArrow (alt : Syntax) : Syntax :=
+  alt[1]
+
+def isHoleRHS (rhs : Syntax) : Bool :=
+  rhs.isOfKind ``Parser.Term.syntheticHole || rhs.isOfKind ``Parser.Term.hole
+
+def evalAlt (mvarId : MVarId) (alt : Syntax) (remainingGoals : Array MVarId) : TacticM (Array MVarId) :=
+  let rhs := getAltRHS alt
+  withCaseRef (getAltDArrow alt) rhs do
+    if isHoleRHS rhs then
+      let gs' ← mvarId.withContext <| withRef rhs do
+        let mvarDecl ← mvarId.getDecl
+        let val ← elabTermEnsuringType rhs mvarDecl.type
+        mvarId.assign val
+        let gs' ← getMVarsNoDelayed val
+        tagUntaggedGoals mvarDecl.userName `induction gs'.toList
+        pure gs'
+      return remainingGoals ++ gs'
+    else
+      setGoals [mvarId]
+      closeUsingOrAdmit (withTacticInfoContext alt (evalTactic rhs))
+      return remainingGoals
+
+structure Context where
+  elimInfo : ElimInfo
+  targets  : Array Expr -- targets provided by the user
+
+structure State where
+  argPos    : Nat := 0 -- current argument position
+  targetPos : Nat := 0 -- current target at targetsStx
+  f         : Expr
+  fType     : Expr
+  alts      : Array (Name × MVarId) := #[]
+  insts     : Array MVarId := #[]
+
+abbrev M := ReaderT Context $ StateRefT State TermElabM
+
+private def addNewArg (arg : Expr) : M Unit :=
+  modify fun s => { s with argPos := s.argPos+1, f := mkApp s.f arg, fType := s.fType.bindingBody!.instantiate1 arg }
+
+private def getBindingName : M Name := return (← get).fType.bindingName!
+private def getArgExpectedType : M Expr := return (← get).fType.bindingDomain!
+
+private def getFType : M Expr := do
+  let fType ← whnfForall (← get).fType
+  modify fun s => { s with fType := fType }
+  pure fType
+
+structure Result where
+  elimApp : Expr
+  alts    : Array (Name × MVarId) := #[]
+  others  : Array MVarId := #[]
+
+partial def mkElimApp (elimInfo : ElimInfo) (targets : Array Expr) (tag : Name) : TermElabM Result := do
+  let rec loop : M Unit := do
+    match (← getFType) with
+    | .forallE binderName _ _ c =>
+      let ctx ← read
+      let argPos := (← get).argPos
+      if ctx.elimInfo.motivePos == argPos then
+        let motive ← mkFreshExprMVar (← getArgExpectedType) MetavarKind.syntheticOpaque
+        addNewArg motive
+      else if ctx.elimInfo.targetsPos.contains argPos then
+        let s ← get
+        let ctx ← read
+        unless s.targetPos < ctx.targets.size do
+          throwError "insufficient number of targets for '{elimInfo.name}'"
+        let target := ctx.targets[s.targetPos]!
+        let expectedType ← getArgExpectedType
+        let target ← withAssignableSyntheticOpaque <| Term.ensureHasType expectedType target
+        modify fun s => { s with targetPos := s.targetPos + 1 }
+        addNewArg target
+      else match c with
+        | .implicit =>
+          let arg ← mkFreshExprMVar (← getArgExpectedType)
+          addNewArg arg
+        | .strictImplicit =>
+          let arg ← mkFreshExprMVar (← getArgExpectedType)
+          addNewArg arg
+        | .instImplicit =>
+          let arg ← mkFreshExprMVar (← getArgExpectedType) (kind := MetavarKind.synthetic) (userName := appendTag tag binderName)
+          modify fun s => { s with insts := s.insts.push arg.mvarId! }
+          addNewArg arg
+        | _ =>
+          let arg ← mkFreshExprSyntheticOpaqueMVar (← getArgExpectedType) (tag := appendTag tag binderName)
+          let x   ← getBindingName
+          modify fun s => { s with alts := s.alts.push (x, arg.mvarId!) }
+          addNewArg arg
+      loop
+    | _ =>
+      pure ()
+  let f ← Term.mkConst elimInfo.name
+  let fType ← inferType f
+  let (_, s) ← (loop).run { elimInfo := elimInfo, targets := targets } |>.run { f := f, fType := fType }
+  let mut others := #[]
+  for mvarId in s.insts do
+    try
+      unless (← Term.synthesizeInstMVarCore mvarId) do
+        mvarId.setKind .syntheticOpaque
+        others := others.push mvarId
+    catch _ =>
+      mvarId.setKind .syntheticOpaque
+      others := others.push mvarId
+  let alts ← s.alts.filterM fun alt => return !(← alt.2.isAssigned)
+  return { elimApp := (← instantiateMVars s.f), alts, others := others }
+
+def setMotiveArg (mvarId : MVarId) (motiveArg : MVarId) (targets : Array FVarId) : MetaM Unit := do
+  let type ← inferType (mkMVar mvarId)
+  let motive ← mkLambdaFVars (targets.map mkFVar) type
+  let motiverInferredType ← inferType motive
+  let motiveType ← inferType (mkMVar motiveArg)
+  unless (← isDefEqGuarded motiverInferredType motiveType) do
+    throwError "type mismatch when assigning motive{indentExpr motive}\n{← mkHasTypeButIsExpectedMsg motiverInferredType motiveType}"
+  motiveArg.assign motive
+
+private def getAltNumFields (elimInfo : ElimInfo) (altName : Name) : TermElabM Nat := do
+  for altInfo in elimInfo.altsInfo do
+    if altInfo.name == altName then
+      return altInfo.numFields
+  throwError "unknown alternative name '{altName}'"
+
+private def checkAltNames (alts : Array (Name × MVarId)) (altsSyntax : Array Syntax) : TacticM Unit :=
+  for i in [:altsSyntax.size] do
+    let altStx := altsSyntax[i]!
+    if getAltName altStx == `_ && i != altsSyntax.size - 1 then
+      withRef altStx <| throwError "invalid occurrence of wildcard alternative, it must be the last alternative"
+    let altName := getAltName altStx
+    if altName != `_ then
+      unless alts.any fun (n, _) => n == altName do
+        throwErrorAt altStx "invalid alternative name '{altName}'"
+
+private def getNumExplicitFields (altMVarId : MVarId) (numFields : Nat) : MetaM Nat := altMVarId.withContext do
+  let target ← altMVarId.getType
+  withoutModifyingState do
+    let (_, bis, _) ← forallMetaBoundedTelescope target numFields
+    return bis.foldl (init := 0) fun r bi => if bi.isExplicit then r + 1 else r
+
+private def saveAltVarsInfo (altMVarId : MVarId) (altStx : Syntax) (fvarIds : Array FVarId) : TacticM Unit :=
+  withSaveInfoContext <| altMVarId.withContext do
+    let useNamesForExplicitOnly := !altHasExplicitModifier altStx
+    let mut i := 0
+    let altVars := getAltVars altStx
+    for fvarId in fvarIds do
+      if !useNamesForExplicitOnly || (← fvarId.getDecl).binderInfo.isExplicit then
+        if i < altVars.size then
+          Term.addLocalVarInfo altVars[i]! (mkFVar fvarId)
+          i := i + 1
+
+def reorderAlts (alts : Array (Name × MVarId)) (altsSyntax : Array Syntax) : Array (Name × MVarId) := Id.run do
+  if altsSyntax.isEmpty then
+    return alts
+  else
+    let mut alts := alts
+    let mut result := #[]
+    for altStx in altsSyntax do
+      let altName := getAltName altStx
+      let some i := alts.findIdx? (·.1 == altName) | return result ++ alts
+      result := result.push alts[i]!
+      alts := alts.eraseIdx i
+    return result ++ alts
+
+private def getUserGeneralizingFVarIds (stx : Syntax) : TacticM (Array FVarId) :=
+  withRef stx do
+    let generalizingStx := stx[3]
+    if generalizingStx.isNone then
+      pure #[]
+    else
+      trace[Elab.induction] "{generalizingStx}"
+      let vars := generalizingStx[1].getArgs
+      getFVarIds vars
+
+private def generalizeVars (mvarId : MVarId) (stx : Syntax) (targets : Array Expr) : TacticM (Nat × MVarId) :=
+  mvarId.withContext do
+    let userFVarIds ← getUserGeneralizingFVarIds stx
+    let forbidden ← mkGeneralizationForbiddenSet targets
+    let mut s ← getFVarSetToGeneralize targets forbidden
+    for userFVarId in userFVarIds do
+      if forbidden.contains userFVarId then
+        throwError "variable cannot be generalized because target depends on it{indentExpr (mkFVar userFVarId)}"
+      if s.contains userFVarId then
+        throwError "unnecessary 'generalizing' argument, variable '{mkFVar userFVarId}' is generalized automatically"
+      s := s.insert userFVarId
+    let fvarIds ← sortFVarIds s.toArray
+    let (fvarIds, mvarId') ← mvarId.revert fvarIds
+    return (fvarIds.size, mvarId')
+
+private def getAltsOfInductionAlts (inductionAlts : Syntax) : Array Syntax :=
+  inductionAlts[2].getArgs
+
+private def getAltsOfOptInductionAlts (optInductionAlts : Syntax) : Array Syntax :=
+  if optInductionAlts.isNone then #[] else getAltsOfInductionAlts optInductionAlts[0]
+
+private def getOptPreTacOfOptInductionAlts (optInductionAlts : Syntax) : Syntax :=
+  if optInductionAlts.isNone then mkNullNode else optInductionAlts[0][1]
+
+private def isMultiAlt (alt : Syntax) : Bool :=
+  alt[0].getNumArgs > 1
+
+/-- Return `some #[alt_1, ..., alt_n]` if `alt` has multiple LHSs. -/
+private def expandMultiAlt? (alt : Syntax) : Option (Array Syntax) := Id.run do
+  if isMultiAlt alt then
+    some <| alt[0].getArgs.map fun lhs => alt.setArg 0 (mkNullNode #[lhs])
+  else
+    none
+
+private def expandInductionAlts? (inductionAlts : Syntax) : Option Syntax := Id.run do
+  let alts := getAltsOfInductionAlts inductionAlts
+  if alts.any isMultiAlt then
+    let mut altsNew := #[]
+    for alt in alts do
+      if let some alt' := expandMultiAlt? alt then
+        altsNew := altsNew ++ alt'
+      else
+        altsNew := altsNew.push alt
+    some <| inductionAlts.setArg 2 (mkNullNode altsNew)
+  else
+    none
+
+private def expandInduction? (induction : Syntax) : Option Syntax := do
+  let optInductionAlts := induction[4]
+  guard <| !optInductionAlts.isNone
+  let inductionAlts' ← expandInductionAlts? optInductionAlts[0]
+  return induction.setArg 4 (mkNullNode #[inductionAlts'])
+
+private def expandCases? (induction : Syntax) : Option Syntax := do
+  let optInductionAlts := induction[3]
+  guard <| !optInductionAlts.isNone
+  let inductionAlts' ← expandInductionAlts? optInductionAlts[0]
+  return induction.setArg 3 (mkNullNode #[inductionAlts'])
+
+private def checkAltsOfOptInductionAlts (optInductionAlts : Syntax) : TacticM Unit :=
+  unless optInductionAlts.isNone do
+    let mut found := false
+    for alt in getAltsOfInductionAlts optInductionAlts[0] do
+      let n := getAltName alt
+      if n == `_ then
+        unless (getAltVarNames alt).isEmpty do
+          throwErrorAt alt "wildcard alternative must not specify variable names"
+        if found then
+          throwErrorAt alt "more than one wildcard alternative '| _ => ...' used"
+        found := true
+
+def getInductiveValFromMajor (major : Expr) : TacticM InductiveVal :=
+  liftMetaMAtMain fun mvarId => do
+    let majorType ← inferType major
+    let majorType ← whnf majorType
+    matchConstInduct majorType.getAppFn
+      (fun _ => Meta.throwTacticEx `induction mvarId m!"major premise type is not an inductive type {indentExpr majorType}")
+      (fun val _ => pure val)
+
+private def getElimNameInfo (optElimId : Syntax) (targets : Array Expr) (induction : Bool): TacticM ElimInfo := do
+  if optElimId.isNone then
+    if let some elimInfo ← getCustomEliminator? targets then
+      return elimInfo
+    unless targets.size == 1 do
+      throwError "eliminator must be provided when multiple targets are used (use 'using <eliminator-name>'), and no default eliminator has been registered using attribute `[eliminator]`"
+    let indVal ← getInductiveValFromMajor targets[0]!
+    if induction && indVal.all.length != 1 then
+      throwError "'induction' tactic does not support mutually inductive types, the eliminator '{mkRecName indVal.name}' has multiple motives"
+    if induction && indVal.isNested then
+      throwError "'induction' tactic does not support nested inductive types, the eliminator '{mkRecName indVal.name}' has multiple motives"
+    let elimName := if induction then mkRecName indVal.name else mkCasesOnName indVal.name
+    getElimInfo elimName
+  else
+    let elimId := optElimId[1]
+    let elimName ← withRef elimId do resolveGlobalConstNoOverloadWithInfo elimId
+    withRef elimId <| getElimInfo elimName
+
+private def shouldGeneralizeTarget (e : Expr) : MetaM Bool := do
+  if let .fvar fvarId .. := e then
+    return (←  fvarId.getDecl).hasValue -- must generalize let-decls
+  else
+    return true
+
+private def generalizeTargets (exprs : Array Expr) : TacticM (Array Expr) := do
+  if (← withMainContext <| exprs.anyM (shouldGeneralizeTarget ·)) then
+    liftMetaTacticAux fun mvarId => do
+      let (fvarIds, mvarId) ← mvarId.generalize (exprs.map fun expr => { expr })
+      return (fvarIds.map mkFVar, [mvarId])
+  else
+    return exprs
+
+def elabCasesTargets (targets : Array Syntax) : TacticM (Array Expr) :=
+  withMainContext do
+    let args ← targets.mapM fun target => do
+      let hName? := if target[0].isNone then none else some target[0][0].getId
+      let expr ← elabTerm target[1] none
+      return { expr, hName? : GeneralizeArg }
+    if (← withMainContext <| args.anyM fun arg => shouldGeneralizeTarget arg.expr <||> pure arg.hName?.isSome) then
+      liftMetaTacticAux fun mvarId => do
+        let argsToGeneralize ← args.filterM fun arg => shouldGeneralizeTarget arg.expr <||> pure arg.hName?.isSome
+        let (fvarIdsNew, mvarId) ← mvarId.generalize argsToGeneralize
+        let mut result := #[]
+        let mut j := 0
+        for arg in args do
+          if (← shouldGeneralizeTarget arg.expr) || arg.hName?.isSome then
+            result := result.push (mkFVar fvarIdsNew[j]!)
+            j := j+1
+          else
+            result := result.push arg.expr
+        return (result, [mvarId])
+    else
+      return args.map (·.expr)
+
+-- # End of duplicate code
+
+def appendMVars (old : Array MVarId) (new : Array MVarId) : TacticM (Array MVarId) := 
+  return old ++ new
+
+-- Resembles `evalAlts` in Core Lean
+def getMVarsFromAlts (elimInfo : ElimInfo) (alts : Array (Name × MVarId)) (optPreTac : Syntax) (altsSyntax : Array Syntax)
+    (initialInfo : Info)
+    (numEqs : Nat := 0) (numGeneralized : Nat := 0) (toClear : Array FVarId := #[]) : TacticM (Array MVarId) := do
+  checkAltNames alts altsSyntax
+  let hasAlts := altsSyntax.size > 0
+  if hasAlts then
+    -- default to initial state outside of alts
+    withInfoContext go (pure initialInfo)
+  else go
+where
+  go := do
+    let alts := reorderAlts alts altsSyntax
+    let hasAlts := altsSyntax.size > 0
+    let mut usedWildcard := false
+    let mut subgoals := #[] -- when alternatives are not provided, we accumulate subgoals here
+    let mut altsSyntax := altsSyntax
+
+    -- TODO foreach, add mvar to list, or alts.mapM
+    let mut mvars : List MVarId := []
     
---     admit -- TODO
+    for (altName, altMVarId) in alts do
+      let numFields ← getAltNumFields elimInfo altName
+      let mut isWildcard := false
+      let altStx? ←
+        match altsSyntax.findIdx? (fun alt => getAltName alt == altName) with
+        | some idx =>
+          let altStx := altsSyntax[idx]!
+          altsSyntax := altsSyntax.eraseIdx idx
+          pure (some altStx)
+        | none => match altsSyntax.findIdx? (fun alt => getAltName alt == `_) with
+          | some idx =>
+            isWildcard := true
+            pure (some altsSyntax[idx]!)
+          | none =>
+            pure none
+      match altStx? with
+      | none =>
+        -- Change: Ignore this match, 
+        -- this is probably a match without any alternative syntax, all intro's are inaccessible anyways
+        let mut (_, altMVarId) ← altMVarId.introN numFields
+        match (← Cases.unifyEqs? numEqs altMVarId {}) with
+        | none   => pure () -- alternative is not reachable
+        | some (altMVarId', _) =>
+          (_, altMVarId) ← altMVarId'.introNP numGeneralized
+          for fvarId in toClear do
+            altMVarId ← altMVarId.tryClear fvarId
+          let altMVarIds ← applyPreTac altMVarId
+          if !hasAlts then
+            -- User did not provide alternatives using `|`
+            subgoals := subgoals ++ altMVarIds.toArray
+          else if altMVarIds.isEmpty then
+            pure ()
+          else
+            logError m!"alternative '{altName}' has not been provided"
+            altMVarIds.forM fun mvarId => admitGoal mvarId
+      | some altStx =>
+        (subgoals, usedWildcard, mvars) ← withRef altStx do
+          let unusedAlt :=
+            if isWildcard then
+              pure (#[], usedWildcard, [])
+            else
+              throwError "alternative '{altName}' is not needed"
+          let altVarNames := getAltVarNames altStx
+          let numFieldsToName ← if altHasExplicitModifier altStx then pure numFields else getNumExplicitFields altMVarId numFields
+          if altVarNames.size > numFieldsToName then
+            logError m!"too many variable names provided at alternative '{altName}', #{altVarNames.size} provided, but #{numFieldsToName} expected"
+          let mut (fvarIds, altMVarId) ← altMVarId.introN numFields altVarNames.toList (useNamesForExplicitOnly := !altHasExplicitModifier altStx)
 
--- def while_intro' {b P Q : state → Prop} {S}
---     (I : state → Prop)
---     (hS : {* fun s => I s ∧ b s *} S {* I *})
---     (hP : ∀s, P s → I s)
---     (hQ : ∀s, ¬ b s → I s → Q s) :
---   {* P *} stmt.while_tmp b S {* Q *} := by admit -- proof omitted
+          saveAltVarsInfo altMVarId altStx fvarIds
+          match (← Cases.unifyEqs? numEqs altMVarId {}) with
+          | none => unusedAlt
+          | some (altMVarId', _) =>
+            (_, altMVarId) ← altMVarId'.introNP numGeneralized
+            for fvarId in toClear do
+              altMVarId ← altMVarId.tryClear fvarId
+            let altMVarIds ← applyPreTac altMVarId
+            if altMVarIds.isEmpty then
+              unusedAlt
+            else
+              let mut subgoals := subgoals
 
--- def ADD : stmt :=
--- stmt.while_tmp (fun s => s "n" ≠ 0)
---   (stmt.assign "n" (fun s => s "n" - 1) ;;
---    stmt.assign "m" (fun s => s "m" + 1))
+              for altMVarId' in altMVarIds do
+                subgoals ← evalAlt altMVarId' altStx subgoals
+              pure (subgoals, usedWildcard || isWildcard, altMVarIds)          
+    if usedWildcard then
+      altsSyntax := altsSyntax.filter fun alt => getAltName alt != `_
+    unless altsSyntax.isEmpty do
+      logErrorAt altsSyntax[0]! "unused alternative"
+    setGoals subgoals.toList
+    -- Change, actually return mvars
+    return mvars.toArray
+  applyPreTac (mvarId : MVarId) : TacticM (List MVarId) :=
+    if optPreTac.isNone then do
+      return [mvarId]
+    else
+      evalTacticAt optPreTac[0] mvarId
 
--- -- TODO, can't get `while_intro'` to work
--- -- theorem ADD_correct (n₀ m₀ : Nat) :
--- --   {* fun s => s "n" = n₀ ∧ s "m" = m₀ *}
--- --   ADD
--- --   {* fun s => s "n" = 0 ∧ s "m" = n₀ + m₀ *} :=
--- --   while_intro (fun s : state => s "n" + s "m" = n₀ + m₀)
--- --   by admit
+-- Resembles `evalCases` in Core Lean
+def getMVarsFromCaseMatch (stx : Syntax) : TacticM (Array MVarId) :=
+  match expandCases? stx with
+  | some stxNew => do
+    -- Changed to ignore macro expansion, since evalTactic does not automatically reduce to a correctly nested call to this function
+    trace[Elab.induction] m!"Current implementation ignores macro expansion"
+    return #[]
+  | _ => focus do
+    let targets ← elabCasesTargets stx[1].getSepArgs
+    let optInductionAlts := stx[3]
+    let optPreTac := getOptPreTacOfOptInductionAlts optInductionAlts
+    let alts :=  getAltsOfOptInductionAlts optInductionAlts
+    let targetRef := stx[1]
+    let elimInfo ← withMainContext <| getElimNameInfo stx[2] targets (induction := false)
+    let mvarId ← getMainGoal
+    let initInfo ← mkTacticInfo (← getMCtx) (← getUnsolvedGoals) (← getRef)
+    let tag ← mvarId.getTag
+    mvarId.withContext do
+      let targets ← addImplicitTargets elimInfo targets
+      let result ← withRef targetRef <| mkElimApp elimInfo targets tag
+      let elimArgs := result.elimApp.getAppArgs
+      let targets ← elimInfo.targetsPos.mapM fun i => instantiateMVars elimArgs[i]!
+      let motiveType ← inferType elimArgs[elimInfo.motivePos]!
+      let mvarId ← generalizeTargetsEq mvarId motiveType targets
+      let (targetsNew, mvarId) ← mvarId.introN targets.size
 
--- inductive small_step : stmt × state → stmt × state → Prop
--- | assign {x a s} :
---   small_step (stmt.assign x a, s) (stmt.skip, s{x ↦ a s})
--- | seq_step {S S' T s s'} (hS : small_step (S, s) (S', s')) :
---   small_step (S ;; T, s) (S' ;; T, s')
--- | seq_skip {T s} :
---   small_step (stmt.skip ;; T, s) (T, s)
--- | ite_true {b : state → Prop} {S T s} (hcond : b s) :
---   small_step (stmt.ite b S T, s) (S, s)
--- | ite_false {b : state → Prop} {S T s} (hcond : ¬ b s) :
---   small_step (stmt.ite b S T, s) (T, s)
--- | while {b : state → Prop} {S s} :
---   small_step (stmt.while_tmp b S, s)
---     (stmt.ite b (S ;; stmt.while_tmp b S) stmt.skip, s)
+      mvarId.withContext do
+        setMotiveArg mvarId elimArgs[elimInfo.motivePos]!.mvarId! targetsNew
+        mvarId.assign result.elimApp
 
--- infixr:60 " ⇒ " => small_step
+        -- Changed call to `evalAlts` to modified version that returns `Array MVarId`
+        return (←  getMVarsFromAlts elimInfo result.alts optPreTac alts initInfo (numEqs := targets.size) (toClear := targetsNew))
 
+-- Resembles `evalInduction` in Core Lean
+-- def 
+def getMVarsFromInductionMatch (stx : Syntax) : TacticM (Array MVarId) := 
+  match expandInduction? stx with
+  | some stxNew => do
+    -- Changed to ignore macro expansion, since evalTactic does not automatically reduce to a correctly nested call to this function
+      trace[Elab.induction] m!"Current implementation ignores macro expansion"
+      return #[]
+  | _ => focus do
+    let optInductionAlts := stx[4]
+    let alts := getAltsOfOptInductionAlts optInductionAlts
+    let targets ← withMainContext <| stx[1].getSepArgs.mapM (elabTerm · none)
+    let targets ← generalizeTargets targets
+    let elimInfo ← withMainContext <| getElimNameInfo stx[2] targets (induction := true)
+    let mvarId ← getMainGoal
+    -- save initial info before main goal is reassigned
+    let initInfo ← mkTacticInfo (← getMCtx) (← getUnsolvedGoals) (← getRef)
+    let tag ← mvarId.getTag
+    mvarId.withContext do
+      let targets ← addImplicitTargets elimInfo targets
+      checkTargets targets
+      let targetFVarIds := targets.map (·.fvarId!)
+      let (n, mvarId) ← generalizeVars mvarId stx targets
+      mvarId.withContext do
+        let result ← withRef stx[1] do -- use target position as reference
+          mkElimApp elimInfo targets tag
+        trace[Elab.induction] "elimApp: {result.elimApp}"
+        let elimArgs := result.elimApp.getAppArgs
+        setMotiveArg mvarId elimArgs[elimInfo.motivePos]!.mvarId! targetFVarIds
+        let optPreTac := getOptPreTacOfOptInductionAlts optInductionAlts
+        mvarId.assign result.elimApp
 
--- example : ¬ p := by
+        -- Changed call to `evalAlts` to modified version that returns `Array MVarId`
+        return (←  getMVarsFromAlts elimInfo result.alts optPreTac alts initInfo (numGeneralized := n) (toClear := targetFVarIds))
+where
+  checkTargets (targets : Array Expr) : MetaM Unit := do
+    let mut foundFVars : FVarIdSet := {}
+    for target in targets do
+      unless target.isFVar do
+        throwError "index in target's type is not a variable (consider using the `cases` tactic instead){indentExpr target}"
+      if foundFVars.contains target.fvarId! then
+        throwError "target (or one of its indices) occurs more than once{indentExpr target}"
 
--- -- Maybe small step semantics better, larger proofs and can do pretty nice annotations here without too much custom notation
--- theorem small_step_final (S s) :
---   (¬ ∃T t, (S, s) ⇒ (T, t)) ↔ S = stmt.skip := by 
---   induction S with 
---   | skip =>
---     simp [Not]
---     intros T t hst
---     admit
+def getMVarsFromMatch (oldGoal : MVarId) (matchTactic : TSyntax `tactic) (isInduction : Bool) : TacticM (Array MVarId) := do
+  withoutModifyingState do 
+    match isInduction with
+    | true => return (← getMVarsFromInductionMatch matchTactic.raw)
+    | false => return (← getMVarsFromCaseMatch matchTactic.raw)
 
---   | assign x a => 
---     simp [Not]
---     apply Exists.intro (fun x => false)
---   | seq S T ihS ihT => sorry
---   | ite b S T ihS ihT => sorry
---   | while_tmp b S ih => sorry
-    
--- begin
---   induction' S,
---   case skip {
---     simp,
---     intros T t hstep,
---     cases' hstep },
---   case assign : x a {
---     simp,
---     apply exists.intro stmt.skip,
---     apply exists.intro (s{x ↦ a s}),
---     exact small_step.assign },
---   case seq : S T ihS ihT {
---     simp,
---     cases' classical.em (S = stmt.skip),
---     case inl {
---       rw h,
---       apply exists.intro T,
---       apply exists.intro s,
---       exact small_step.seq_skip },
---     case inr {
---       simp [h, auto.not_forall_eq, auto.not_not_eq] at ihS,
---       cases' ihS s with S' hS',
---       cases' hS' with s' hs',
---       apply exists.intro (S' ;; T),
---       apply exists.intro s',
---       exact small_step.seq_step hs' } },
---   case ite : b S T ihS ihT {
---     simp,
---     cases' classical.em (b s),
---     case inl {
---       apply exists.intro S,
---       apply exists.intro s,
---       exact small_step.ite_true h },
---     case inr {
---       apply exists.intro T,
---       apply exists.intro s,
---       exact small_step.ite_false h } },
---   case while : b S ih {
---     simp,
---     apply exists.intro (stmt.ite b (S ;; stmt.while b S) stmt.skip),
---     apply exists.intro s,
---     exact small_step.while }
--- end
-end LoVe
-
-
-example : α → β ∧ γ → α ∧ β := by
-  intros ha hbg
-  have hb : β := hbg.left
-  exact And.intro ha hb
-
-example : α → β ∧ γ → α ∧ β := by
-  fix (ha : α) (hbg : β ∧ γ) ⊢ α ∧ β -- fix always uses intros
-  have hb : β := hbg.left
-  exact And.intro ha hb
-
-example : α → β ∧ γ → α ∧ β := by
-  note (ha : α) (hbg : β ∧ γ) (hb : β) ⊢ α ∧ β by
-    intros ha hbg
-    have hb : β := hbg.left
-  exact And.intro ha hb
-
-example : α → β ∧ γ → α ∧ β := by
-  intros ha hbg
-  have hb : β := hbg.left
-  show α ∧ β by 
-    exact And.intro ha hb
-
-
-example (n : Nat) : true := by
-  cases n with
-  | zero => 
-    rfl
-  | succ n => 
-    rfl
-
-example (n : Nat) : true := by
-  induction n with
-  | zero => 
-    rfl
-  | succ n ih => 
-    rfl
-
-
--- Already declared in Struct for testing
--- inductive Even : Nat → Prop
--- | zero : Even Nat.zero
--- | add_two : ∀ k : Nat, Even k → Even (k+2) 
+end InductionHelper
